src/rocq/Semantics/IntrinsicsDefinitions.v
@@ -375,8 +375,9 @@ Section Intrinsics.
 
    - The right-hand [dvalue] of the [+] result is used to throw an exception.
    *)
-  Definition pure_function     := list dvalue -> EOU (dvalue + dvalue).
-  Definition semantic_function := list dvalue -> option ptr -> itree E (dvalue + dvalue).
+  Definition pure_base_function := list dvalue_base -> EOU (dvalue_base + dvalue_base).
+  Definition pure_function      := list dvalue -> EOU (dvalue + dvalue).
+  Definition semantic_function  := list dvalue -> option ptr -> itree E (dvalue + dvalue).
 
   (* An association list mapping intrinsic names to their semantic definitions *)
   Definition intrinsic_definitions := list (declaration typ * semantic_function).
@@ -386,7 +387,7 @@ Section Intrinsics.
 
   #[local] Notation retr x := (ret (inr x)).
   (* Absolute value for Float. *)
-  Definition llvm_fabs_f32 : pure_function :=
+  Definition llvm_fabs_f32 : pure_base_function :=
     fun args =>
       match args with
       | [DVALUE_Float d] => retr (DVALUE_Float (b32_abs d))
@@ -394,7 +395,7 @@ Section Intrinsics.
       end.
 
   (* Abosulute value for Doubles. *)
-  Definition llvm_fabs_f64 : pure_function :=
+  Definition llvm_fabs_f64 : pure_base_function :=
     fun args =>
       match args with
       | [DVALUE_Double d] => retr (DVALUE_Double (b64_abs d))
@@ -415,14 +416,14 @@ Section Intrinsics.
       if Float32.cmp Clt a b then b else a
     end.
 
-  Definition llvm_maxnum_f64 : pure_function :=
+  Definition llvm_maxnum_f64 : pure_base_function :=
     fun args =>
       match args with
       | [DVALUE_Double a; DVALUE_Double b] => retr (DVALUE_Double (Float_maxnum a b))
       | _ => raise_error "llvm_maxnum_f64 got incorrect / ill-typed inputs"
       end.
 
-  Definition llvm_maxnum_f32 : pure_function :=
+  Definition llvm_maxnum_f32 : pure_base_function :=
     fun args =>
       match args with
       | [DVALUE_Float a; DVALUE_Float b] => retr (DVALUE_Float (Float32_maxnum a b))
@@ -443,14 +444,14 @@ Section Intrinsics.
       if Float32.cmp Clt a b then a else b
     end.
 
-  Definition llvm_minimum_f64 : pure_function :=
+  Definition llvm_minimum_f64 : pure_base_function :=
     fun args =>
       match args with
       | [DVALUE_Double a; DVALUE_Double b] => retr (DVALUE_Double (Float_minimum a b))
       | _ => raise_error "llvm_minimum_f64 got incorrect / ill-typed inputs"
       end.
 
-  Definition llvm_minimum_f32 : pure_function :=
+  Definition llvm_minimum_f32 : pure_base_function :=
     fun args =>
       match args with
       | [DVALUE_Float a; DVALUE_Float b] => retr (DVALUE_Float (Float32_minimum a b))
@@ -458,7 +459,7 @@ Section Intrinsics.
       end.
 
   (* Saturated arithmetic: https://llvm.org/docs/LangRef.html#saturation-arithmetic-intrinsics *)
-  Definition ushl_sat {I : Type} `{TDI : ToDvalue I} `{VMI : VMemInt I} (x y : I) : EOU dvalue :=
+  Definition ushl_sat {I : Type} `{TDI : ToDvalueBase I} `{VMI : VMemInt I} (x y : I) : EOU dvalue_base :=
     res <- mshl x y;;
     let res_u := munsigned res in
     let res_u' := Z.shiftl (munsigned x) (munsigned y) in
@@ -475,47 +476,47 @@ Section Intrinsics.
             | raise_oom _ =>
                 raise_error "ushl_sat: cannot represent maximum value in type... Should not happen."
             (* Note: we have enlarged the monad, so that statically we don't rule out new absurd cases such as failure or ub *)
-            | m => to_dvalue <$> m
+            | m => tdb <$> m
             end
         end
-      else ret (to_dvalue res).
+      else ret (tdb res).
 
-  Definition llvm_ushl_sat_1: pure_function :=
+  Definition llvm_ushl_sat_1: pure_base_function :=
     fun args =>
       match args with
       | [DVALUE_I 1 a; DVALUE_I 1 b] => inr <$> ushl_sat a b
       | _ => raise_error "llvm_ushl_sat_1 got incorrect / ill-typed inputs"
       end.
 
-  Definition llvm_ushl_sat_8: pure_function :=
+  Definition llvm_ushl_sat_8: pure_base_function :=
     fun args =>
       match args with
       | [DVALUE_I 8 a; DVALUE_I 8 b] => inr <$> ushl_sat a b
       | _ => raise_error "llvm_ushl_sat_8 got incorrect / ill-typed inputs"
       end.
 
-  Definition llvm_ushl_sat_16: pure_function :=
+  Definition llvm_ushl_sat_16: pure_base_function :=
     fun args =>
       match args with
       | [DVALUE_I 16 a; DVALUE_I 16 b] => inr <$> ushl_sat a b
       | _ => raise_error "llvm_ushl_sat_16 got incorrect / ill-typed inputs"
       end.
 
-  Definition llvm_ushl_sat_32: pure_function :=
+  Definition llvm_ushl_sat_32: pure_base_function :=
     fun args =>
       match args with
       | [DVALUE_I 32 a; DVALUE_I 32 b] => inr <$> ushl_sat a b
       | _ => raise_error "llvm_ushl_sat_32 got incorrect / ill-typed inputs"
       end.
 
-  Definition llvm_ushl_sat_64: pure_function :=
+  Definition llvm_ushl_sat_64: pure_base_function :=
     fun args =>
       match args with
       | [DVALUE_I 64 a; DVALUE_I 64 b] => inr <$> ushl_sat a b
       | _ => raise_error "llvm_ushl_sat_64 got incorrect / ill-typed inputs"
       end.
 
-  Definition llvm_vellvm_internal_throw : pure_function :=
+  Definition llvm_vellvm_internal_throw : pure_base_function :=
     fun args =>
       match args with
       (* Raise: the [inl] branch of the intrinsic's [exc + dvalue] result is
@@ -530,9 +531,9 @@ Section Intrinsics.
       match args, varargs with
     | [ a ], Some varargs =>
         match a with
-        | DVALUE_Poison dt => raiseUB ("Store to poisoned address in va_start.")
-        | _ => store DTYPE_Pointer a (DVALUE_Addr varargs);;
-              retr DVALUE_None
+        | DVALUE_Base (DVALUE_Poison dt) => raiseUB ("Store to poisoned address in va_start.")
+        | _ => store DTYPE_Pointer a (DVALUE_Pointer varargs);;
+              retr (DVALUE_Base DVALUE_None)
         end
     | _, _ => raise "va_start: invalid arguments."
     end.
@@ -543,32 +544,44 @@ Section Intrinsics.
       | [dest; src] =>
           vargs <- load DTYPE_Pointer src;;
           store DTYPE_Pointer dest vargs;;
-          retr DVALUE_None
+          retr (DVALUE_Base DVALUE_None)
       | _ => raise ": va_copy invalid arguments"
       end.
 
   Definition llvm_va_end  : semantic_function :=
     fun args varargs =>
-      retr DVALUE_None.
+      retr (DVALUE_Base DVALUE_None).
 
+  Definition pure_base_to_pure : pure_base_function -> pure_function :=
+    fun f args =>
+      args' <- map_monad dvalue_to_dvalue_base args ;;
+      ans <- f args' ;;
+      match ans with
+      | inr x => retr (DVALUE_Base x)
+      | inl x => ret (inl (DVALUE_Base x))
+      end.
+  
   Definition pure_to_semantic : pure_function -> semantic_function :=
     fun f args _ => EOU_to_itree (f args).
 
+  Definition pure_base_to_semantic : pure_base_function -> semantic_function :=
+    fun f => pure_to_semantic (pure_base_to_pure f).
+  
   (* Clients of Vellvm can register the names of their own intrinsics
      definitions here. *)
   Definition defined_intrinsics : intrinsic_definitions :=
-    [ (fabs_32_decl, pure_to_semantic llvm_fabs_f32) ;
-      (fabs_64_decl, pure_to_semantic llvm_fabs_f64) ;
-      (maxnum_32_decl , pure_to_semantic llvm_maxnum_f32) ;
-      (maxnum_64_decl , pure_to_semantic llvm_maxnum_f64);
-      (minimum_32_decl, pure_to_semantic llvm_minimum_f32);
-      (minimum_64_decl, pure_to_semantic llvm_minimum_f64);
-      (ushl_sat_1_decl, pure_to_semantic llvm_ushl_sat_1);
-      (ushl_sat_8_decl, pure_to_semantic llvm_ushl_sat_8);
-      (ushl_sat_16_decl, pure_to_semantic llvm_ushl_sat_16);
-      (ushl_sat_32_decl, pure_to_semantic llvm_ushl_sat_32);
-      (ushl_sat_64_decl, pure_to_semantic llvm_ushl_sat_64);
-      (vellvm_internal_throw_decl, pure_to_semantic llvm_vellvm_internal_throw);
+    [ (fabs_32_decl, pure_base_to_semantic llvm_fabs_f32) ;
+      (fabs_64_decl, pure_base_to_semantic llvm_fabs_f64) ;
+      (maxnum_32_decl , pure_base_to_semantic llvm_maxnum_f32) ;
+      (maxnum_64_decl , pure_base_to_semantic llvm_maxnum_f64);
+      (minimum_32_decl, pure_base_to_semantic llvm_minimum_f32);
+      (minimum_64_decl, pure_base_to_semantic llvm_minimum_f64);
+      (ushl_sat_1_decl, pure_base_to_semantic llvm_ushl_sat_1);
+      (ushl_sat_8_decl, pure_base_to_semantic llvm_ushl_sat_8);
+      (ushl_sat_16_decl, pure_base_to_semantic llvm_ushl_sat_16);
+      (ushl_sat_32_decl, pure_base_to_semantic llvm_ushl_sat_32);
+      (ushl_sat_64_decl, pure_base_to_semantic llvm_ushl_sat_64);
+      (vellvm_internal_throw_decl, pure_base_to_semantic llvm_vellvm_internal_throw);
       (va_start_decl, llvm_va_start);
       (va_end_decl, llvm_va_end);
       (va_copy_decl, llvm_va_copy)
